add whole_prog_spec2 alternative to whole_prog_spec

basis/basis_ffiScript.sml
@@ -458,6 +458,15 @@ val whole_prog_ffidiv_spec_def = Define`
       (POSTf n. λc b. STDIO fs' * RUNTIME * &(n = n' /\ c = c' /\ b = b')) ∧
     post n' c' b' (fs' with numchars := fs.numchars)`;
 
+val whole_prog_spec2_def = Define`
+  whole_prog_spec2 fv cl fs sprop post ⇔
+    app (basis_proj1, basis_proj2) fv [Conv NONE []]
+      (COMMANDLINE cl * STDIO fs * case sprop of NONE => &T | SOME p => p)
+      (POSTv uv. &UNIT_TYPE () uv *
+      SEP_EXISTS fs'.
+        STDIO fs' * &(post (fs' with numchars := fs.numchars))
+      )`;
+
 Theorem whole_prog_spec_semantics_prog:
    ∀fname fv.
      Decls env1 (init_state (basis_ffi cl fs)) prog env2 st2 ==>
@@ -542,6 +551,59 @@ Proof
   \\ `n = n' /\ c = c' /\ b = b'` by(fs[STAR_def,cond_def])
   \\ rveq
   \\ `∃ll. SND st3.ffi.ffi_state = fs' with numchars := ll` suffices_by ( rw[] \\ rw[] )
+  \\ fs[STDIO_def, IOFS_def,cfHeapsBaseTheory.IO_def,
+        cfHeapsBaseTheory.IOx_def, set_sepTheory.SEP_CLAUSES,
+        set_sepTheory.SEP_EXISTS_THM, fsFFITheory.fs_ffi_part_def]
+  \\ fs[GSYM set_sepTheory.STAR_ASSOC]
+  \\ fs[Once STAR_def]
+  \\ fs[set_sepTheory.one_STAR]
+  \\ qmatch_assum_abbrev_tac`one ffip _`
+  \\ fs[one_def]
+  \\ `ffip ∈ (st2heap (basis_proj1,basis_proj2) st3)` by cfHeapsBaseLib.SPLIT_TAC
+  \\ fs [cfStoreTheory.st2heap_def, cfStoreTheory.FFI_part_NOT_IN_store2heap,
+         Abbr`ffip`,cfStoreTheory.ffi2heap_def]
+  \\ Cases_on `parts_ok st3.ffi (basis_proj1, basis_proj2)`
+  \\ fs[FLOOKUP_DEF, MAP_MAP_o, n2w_ORD_CHR_w2n, basis_proj1_write]
+  \\ FIRST_X_ASSUM(ASSUME_TAC o Q.SPEC`"write"`)
+  \\ fs[basis_proj1_write,STAR_def,cond_def]
+  \\ metis_tac[]
+QED
+
+Theorem whole_prog_spec2_semantics_prog:
+   ∀fname fv.
+     Decls env1 (init_state (basis_ffi cl fs)) prog env2 st2 ==>
+     lookup_var fname env2 = SOME fv ==>
+     whole_prog_spec2 fv cl fs sprop Q ==>
+     (?h1 h2. SPLIT (st2heap (basis_proj1, basis_proj2) st2) (h1,h2) /\
+     (COMMANDLINE cl * STDIO fs * case sprop of NONE => &T | SOME Q => Q) h1)
+   ==>
+   ∃io_events fs'.
+     semantics_prog (init_state (basis_ffi cl fs)) env1
+       (SNOC ^main_call prog) (Terminate Success io_events) /\
+     extract_fs fs io_events = SOME fs' ∧ Q fs'
+Proof
+  rw[whole_prog_spec2_def]
+  \\ drule (GEN_ALL call_main_thm2)
+  \\ rpt(disch_then drule)
+  \\ disch_then (qspecl_then [`h2`, `h1`] mp_tac)
+  \\ impl_keep_tac
+  >- (
+    rw[STDIO_def]
+    \\ ho_match_mp_tac FFI_part_hprop_SEP_EXISTS
+    \\ strip_tac
+    \\ match_mp_tac FFI_part_hprop_STAR \\ disj1_tac
+    \\ match_mp_tac FFI_part_hprop_STAR \\ disj1_tac
+    \\ ho_match_mp_tac FFI_part_hprop_SEP_EXISTS
+    \\ metis_tac[IOFS_FFI_part_hprop] )
+  \\ rw[]
+  \\ asm_exists_tac \\ rw[]
+  \\ rw[extract_fs_def,PULL_EXISTS]
+  \\ drule RTC_call_FFI_rel_IMP_basis_events
+  \\ simp[Once ml_progTheory.init_state_def,Once basis_ffi_def]
+  \\ simp[Once ml_progTheory.init_state_def,Once basis_ffi_def]
+  \\ simp[Once extract_fs_with_numchars_def]
+  \\ simp[Once ml_progTheory.init_state_def]
+  \\ rw[basis_proj1_write,Once basis_ffi_def]
   \\ fs[STDIO_def, IOFS_def,cfHeapsBaseTheory.IO_def,
         cfHeapsBaseTheory.IOx_def, set_sepTheory.SEP_CLAUSES,
         set_sepTheory.SEP_EXISTS_THM, fsFFITheory.fs_ffi_part_def]
